{
 "cells": [
  {
   "cell_type": "markdown",
   "id": "f376bad6-b37b-4cb2-a5d0-1dd201fe0487",
   "metadata": {},
   "source": [
    "# Assignment - Recursion Relation"
   ]
  },
  {
   "cell_type": "markdown",
   "id": "5cbf8d6a-6ab7-4bdc-817e-de25719480c5",
   "metadata": {},
   "source": [
    "#1\n",
    "T(2) = 3 . T(1) + 12 . 2 \n",
    "\n",
    "T(1) = 3 . T(0) + 12 . 1 \n",
    "\n",
    "T(0) = 5 \n",
    "\n",
    "T(1) = 3 . 5 + 12 . 1 = 15 + 12 = 27 \n",
    "\n",
    "T(2) = 3 . 27 + 12 . 2 = 81 + 24 = 105 "
   ]
  },
  {
   "cell_type": "markdown",
   "id": "6b0fdacc-4157-467c-b1ef-3f008fcd42ee",
   "metadata": {},
   "source": [
    "#2\n",
    "#a\n",
    "Let's solve the recurrence relation T(n) = T(n-1) + c using the substitution method:\n",
    "\n",
    "1. Assume a solution of the form T(n) = A . n + B\n",
    "2. Substitute the assumed solution into the recurrence relation.\n",
    "3. Solve for the constants A and B.\n",
    "\n",
    "T(n) = T(n-1) + c \n",
    "A . n + B = A . (n-1) + B + c \n",
    "A . n + B = A . n - A + B + c \n",
    "A = c\n",
    "\n",
    "The solution is T(n) = c . n + B"
   ]
  },
  {
   "cell_type": "markdown",
   "id": "e98e92a0-eeee-42a3-b379-f85e3a8f323d",
   "metadata": {},
   "source": [
    "#2\n",
    "#b\n",
    "Let's solve the recurrence relation T(n) = 2T(n/2) + n using the substitution method:\n",
    "\n",
    "1. Substitute T(n) = 2T(n/2) + n\n",
    "2. Substitute T(n/2) = 2T(n/4) + n/2 into the equation\n",
    "3. Repeat the substitution process until a pattern emerges\n",
    "\n",
    "Step 1:\n",
    "T(n) = 2T(n/2) + n\n",
    "\n",
    "Step 2:\n",
    "T(n) = 2(2T(n/4) + n/2) + n = 4T(n/4) + 2n\n",
    "\n",
    "Step 3:\n",
    "T(n) = 2^k T(n/2^k) + kn \n",
    "\n",
    "Repeat until n/2^k = 1:\n",
    "n/2^k = 1 implies k = log_2 n \n",
    "\n",
    "Final solution:\n",
    "T(n) = 2^{log_2 n} T(1) + n log_2 n \n",
    "\n",
    "Simplify using the fact that 2^{log_2 n} = n:\n",
    "T(n) = nT(1) + n log_2 n \n",
    "\n",
    "Simplify further using T(1):\n",
    "T(n) = nT(1) + n log_2 n \n",
    "\n",
    "Thus, the solution to the recurrence relation is:\n",
    "T(n) = nT(1) + n log_2 n"
   ]
  },
  {
   "cell_type": "markdown",
   "id": "65dd44b8-94db-48ed-8073-a980221c2807",
   "metadata": {},
   "source": [
    "#2\n",
    "#c\n",
    "1. Let's start with the given recurrence relation:\n",
    "   T(n) = 2T(n/2) + c\n",
    "\n",
    "2. Make a substitution: n = 2^k, where k = log_2{n}.\n",
    "   T(2^k) = 2T(2^{k-1}) + c \n",
    "\n",
    "3. Substitute T(2^{k-1}) with 2T(2^{k-2}) + c:\n",
    "   T(2^k) = 2(2T(2^{k-2}) + c) + c \n",
    "\n",
    "4. Simplify the expression:\n",
    "   T(2^k) = 2^2T(2^{k-2}) + 2c + c\n",
    "\n",
    "5. Generalize the pattern:\n",
    "   T(2^k) = 2^iT(2^{k-i}) + ic\n",
    "\n",
    "6. When i = k:\n",
    "   T(2^k) = 2^kT(1) + kc\n",
    "\n",
    "7. Substitute back n = 2^k and k = log_2{n}:\n",
    "   T(n) = 2^{log_2{n}}T(1) + log_2{n}c\n",
    "\n",
    "8. Simplify further:\n",
    "   T(n) = nT(1) + log_2{n}c\n",
    "\n",
    "9. If T(1) = c_1, where c_1 is a constant:\n",
    "   T(n) = c_1n + log_2{n}c "
   ]
  },
  {
   "cell_type": "markdown",
   "id": "556776e1-aba0-47db-a789-6e297871b9b3",
   "metadata": {},
   "source": [
    "#2\n",
    "#d\n",
    "1. Assume n = 2^k, where k = log_2{n}.\n",
    "2. Substitute n = 2^k into the recurrence relation:\n",
    "\n",
    "T(2^k) = T(2^{k-1}) + c\n",
    "\n",
    "3. Substitute T(2^{k-1}) with T(2^{k-2}) + c:\n",
    "\n",
    "T(2^k) = (T(2^{k-2}) + c) + c\n",
    "\n",
    "4. Continue substituting until you reach the base case:\n",
    "\n",
    "T(2^k) = T(2^{k-i}) + i . c \n",
    "\n",
    "5. Set T(1) (base case):\n",
    "\n",
    "T(1) = T(2^{k-k}) + k . c\n",
    "\n",
    "6. Simplify:\n",
    "\n",
    "T(1) = T(1) + k . c \n",
    "\n",
    "7. Solve for T(1):\n",
    "\n",
    "T(1) = k . c\n",
    "\n",
    "8. Substitute back k = log_2{n}:\n",
    "\n",
    "T(n) = log_2{n} . c"
   ]
  },
  {
   "cell_type": "markdown",
   "id": "8b28106a-0efe-483f-8109-addb6dbb9976",
   "metadata": {},
   "source": [
    "#3\n",
    "#a\n",
    "\n",
    "          T(n)\n",
    "           |\n",
    "     -----------------\n",
    "     |               |\n",
    "  2T(n-1)           1\n",
    "     |\n",
    "  ---------------\n",
    "  |             |\n",
    "2T(n-2)         1\n",
    "  |\n",
    "  -----------------\n",
    "  |               |\n",
    "2T(n-3)           1\n",
    "  |\n",
    "   ...\n",
    "\n",
    "\n",
    "**Recursive Tree:**\n",
    "\n",
    "1. T(n) = 2T(n-1) + 1\n",
    "\n",
    "**Recursive Tree Steps:**\n",
    "\n",
    "1. Level 0: T(n)\n",
    "2. Level 1: 2T(n-1), 1\n",
    "3. Level 2: 2[2T(n-2), 1] + 1\n",
    "4. Level 3: 2[2[2T(n-3), 1], 1] + 1\n",
    "5. ...\n",
    "\n",
    "**Solving Steps:**\n",
    "\n",
    "1. T(n) = 2T(n-1) + 1\n",
    "2. Substitute T(n-1) with 2T(n-2) + 1:\n",
    "   T(n) = 2[2T(n-2) + 1] + 1\n",
    "3. Simplify:\n",
    "   T(n) = 4T(n-2) + 2 + 1\n",
    "4. Substitute T(n-2) with 2T(n-3) + 1:\n",
    "   T(n) = 4[2T(n-3) + 1] + 2 + 1\n",
    "5. Simplify:\n",
    "   T(n) = 8T(n-3) + 4 + 2 + 1\n",
    "6. ...\n",
    "\n",
    "**General Form:**\n",
    "\n",
    "T(n) = 2^k * T(n-k) + 2^(k-1) + 2^(k-2) + ... + 2 + 1\n",
    "\n",
    "**Base Case:**\n",
    "\n",
    "When n - k = 1, T(1) = 1\n",
    "\n",
    "**Final Answer:**\n",
    "\n",
    "T(n) = 2^n - 1"
   ]
  },
  {
   "cell_type": "markdown",
   "id": "ecb34ca3-a5e4-4cc6-aa69-8fc8e982c639",
   "metadata": {},
   "source": [
    "#3\n",
    "#b\n",
    "1. T(n) = 2T(n/2) + n\n",
    "\n",
    "   Level 1:\n",
    "        T(n)\n",
    "        / \\\n",
    "   T(n/2)  T(n/2) + n\n",
    "\n",
    "   Level 2:\n",
    "        T(n/2)                  T(n/2) + n\n",
    "       /    \\                 /           \\\n",
    "  T(n/4)  T(n/4) + n/2   T(n/4)        T(n/4) + n/2\n",
    "\n",
    "   Level 3:\n",
    "           ...\n",
    "\n",
    "   Level k:\n",
    "           ...\n",
    "\n",
    "2. Expand each node until reaching base case or a constant term:\n",
    "\n",
    "   Level 1:\n",
    "        T(n)\n",
    "        / \\\n",
    "   2T(n/2)  n\n",
    "\n",
    "   Level 2:\n",
    "        2T(n/2)                           T(n/2) + n\n",
    "       /      \\                          /           \\\n",
    "   4T(n/4)   n/2 + T(n/4)           T(n/4)          n/2\n",
    "\n",
    "   Level 3:\n",
    "           ...\n",
    "\n",
    "   Level k:\n",
    "           ...\n",
    "\n",
    "3. Continue expanding until reaching base case:\n",
    "\n",
    "   Level 1:\n",
    "        T(n)\n",
    "        / \\\n",
    "   2T(n/2)  n\n",
    "\n",
    "   Level 2:\n",
    "        2T(n/2)\n",
    "       /      \\\n",
    "   4T(n/4)   n/2 + T(n/4)\n",
    "\n",
    "   Level 3:\n",
    "                ...\n",
    "              /       \\\n",
    "   Level k-1:         T(1)  +  T(1)\n",
    "                          /        \\\n",
    "\n",
    "4. Replace T(1) with its constant value:\n",
    "\n",
    "   Level 1:\n",
    "        T(n)\n",
    "        / \\\n",
    "   2T(n/2)  n\n",
    "\n",
    "   Level 2:\n",
    "        2T(n/2)\n",
    "       /      \\\n",
    "   4T(n/4)   n/2 + 2\n",
    "\n",
    "   Level 3:\n",
    "                ...\n",
    "              /       \\\n",
    "   Level k-1:         1     +      1\n",
    "\n",
    "5. Simplify each level:\n",
    "\n",
    "   Level 1:\n",
    "        T(n)\n",
    "        / \\\n",
    "   2T(n/2)  n\n",
    "\n",
    "   Level 2:\n",
    "        2T(n/2)\n",
    "       /      \\\n",
    "   4T(n/4)   n/2 + 2\n",
    "\n",
    "   Level 3:\n",
    "                ...\n",
    "              /       \\\n",
    "   Level k-1:           2\n",
    "\n",
    "6. Write the final solution:\n",
    "\n",
    "   T(n) = n log n + n"
   ]
  }
 ],
 "metadata": {
  "kernelspec": {
   "display_name": "Python 3 (ipykernel)",
   "language": "python",
   "name": "python3"
  },
  "language_info": {
   "codemirror_mode": {
    "name": "ipython",
    "version": 3
   },
   "file_extension": ".py",
   "mimetype": "text/x-python",
   "name": "python",
   "nbconvert_exporter": "python",
   "pygments_lexer": "ipython3",
   "version": "3.11.6"
  }
 },
 "nbformat": 4,
 "nbformat_minor": 5
}
